examples/proofs/tests/generated_code.v
@@ -6,77 +6,101 @@ Set Default Proof Using "Type".
 (* Generated from [examples/tests.c]. *)
 Section code.
   Definition file_0 : string := "examples/tests.c".
-  Definition loc_2 : location_info := LocationInfo file_0 5 2 5 19.
-  Definition loc_3 : location_info := LocationInfo file_0 6 2 6 13.
-  Definition loc_4 : location_info := LocationInfo file_0 7 2 7 12.
-  Definition loc_5 : location_info := LocationInfo file_0 8 2 8 14.
-  Definition loc_6 : location_info := LocationInfo file_0 9 2 9 13.
-  Definition loc_7 : location_info := LocationInfo file_0 11 2 11 21.
-  Definition loc_8 : location_info := LocationInfo file_0 12 2 12 21.
-  Definition loc_9 : location_info := LocationInfo file_0 13 2 13 21.
-  Definition loc_10 : location_info := LocationInfo file_0 14 2 14 21.
-  Definition loc_11 : location_info := LocationInfo file_0 15 2 15 21.
-  Definition loc_12 : location_info := LocationInfo file_0 17 2 17 17.
-  Definition loc_13 : location_info := LocationInfo file_0 18 2 18 16.
-  Definition loc_14 : location_info := LocationInfo file_0 19 2 19 16.
-  Definition loc_15 : location_info := LocationInfo file_0 20 2 20 16.
-  Definition loc_16 : location_info := LocationInfo file_0 21 2 21 16.
-  Definition loc_17 : location_info := LocationInfo file_0 23 2 23 9.
-  Definition loc_19 : location_info := LocationInfo file_0 21 9 21 16.
-  Definition loc_22 : location_info := LocationInfo file_0 21 5 21 7.
-  Definition loc_24 : location_info := LocationInfo file_0 21 6 21 7.
-  Definition loc_25 : location_info := LocationInfo file_0 21 6 21 7.
-  Definition loc_26 : location_info := LocationInfo file_0 20 9 20 16.
-  Definition loc_29 : location_info := LocationInfo file_0 20 5 20 7.
-  Definition loc_31 : location_info := LocationInfo file_0 20 6 20 7.
-  Definition loc_32 : location_info := LocationInfo file_0 20 6 20 7.
-  Definition loc_33 : location_info := LocationInfo file_0 19 9 19 16.
-  Definition loc_36 : location_info := LocationInfo file_0 19 5 19 7.
-  Definition loc_38 : location_info := LocationInfo file_0 19 6 19 7.
-  Definition loc_39 : location_info := LocationInfo file_0 19 6 19 7.
-  Definition loc_40 : location_info := LocationInfo file_0 18 9 18 16.
-  Definition loc_43 : location_info := LocationInfo file_0 18 5 18 7.
-  Definition loc_45 : location_info := LocationInfo file_0 18 6 18 7.
-  Definition loc_46 : location_info := LocationInfo file_0 18 6 18 7.
-  Definition loc_47 : location_info := LocationInfo file_0 17 10 17 17.
-  Definition loc_50 : location_info := LocationInfo file_0 17 5 17 8.
-  Definition loc_52 : location_info := LocationInfo file_0 17 6 17 8.
-  Definition loc_53 : location_info := LocationInfo file_0 17 6 17 8.
-  Definition loc_54 : location_info := LocationInfo file_0 15 14 15 21.
-  Definition loc_57 : location_info := LocationInfo file_0 15 5 15 12.
-  Definition loc_58 : location_info := LocationInfo file_0 15 5 15 7.
-  Definition loc_59 : location_info := LocationInfo file_0 15 5 15 7.
-  Definition loc_60 : location_info := LocationInfo file_0 15 11 15 12.
-  Definition loc_61 : location_info := LocationInfo file_0 15 11 15 12.
-  Definition loc_62 : location_info := LocationInfo file_0 14 14 14 21.
-  Definition loc_65 : location_info := LocationInfo file_0 14 5 14 12.
-  Definition loc_66 : location_info := LocationInfo file_0 14 5 14 7.
-  Definition loc_67 : location_info := LocationInfo file_0 14 5 14 7.
-  Definition loc_68 : location_info := LocationInfo file_0 14 11 14 12.
-  Definition loc_69 : location_info := LocationInfo file_0 14 11 14 12.
-  Definition loc_70 : location_info := LocationInfo file_0 13 14 13 21.
-  Definition loc_73 : location_info := LocationInfo file_0 13 5 13 12.
-  Definition loc_74 : location_info := LocationInfo file_0 13 5 13 7.
-  Definition loc_75 : location_info := LocationInfo file_0 13 5 13 7.
-  Definition loc_76 : location_info := LocationInfo file_0 13 11 13 12.
-  Definition loc_77 : location_info := LocationInfo file_0 13 11 13 12.
-  Definition loc_78 : location_info := LocationInfo file_0 12 14 12 21.
-  Definition loc_81 : location_info := LocationInfo file_0 12 5 12 12.
-  Definition loc_82 : location_info := LocationInfo file_0 12 5 12 7.
-  Definition loc_83 : location_info := LocationInfo file_0 12 5 12 7.
-  Definition loc_84 : location_info := LocationInfo file_0 12 11 12 12.
-  Definition loc_85 : location_info := LocationInfo file_0 12 11 12 12.
-  Definition loc_86 : location_info := LocationInfo file_0 11 14 11 21.
-  Definition loc_89 : location_info := LocationInfo file_0 11 5 11 12.
-  Definition loc_90 : location_info := LocationInfo file_0 11 5 11 7.
-  Definition loc_91 : location_info := LocationInfo file_0 11 5 11 7.
-  Definition loc_92 : location_info := LocationInfo file_0 11 11 11 12.
-  Definition loc_93 : location_info := LocationInfo file_0 11 11 11 12.
-  Definition loc_94 : location_info := LocationInfo file_0 9 11 9 12.
-  Definition loc_97 : location_info := LocationInfo file_0 8 12 8 13.
-  Definition loc_100 : location_info := LocationInfo file_0 7 10 7 11.
-  Definition loc_103 : location_info := LocationInfo file_0 6 11 6 12.
-  Definition loc_106 : location_info := LocationInfo file_0 5 17 5 18.
+  Definition loc_2 : location_info := LocationInfo file_0 7 2 7 19.
+  Definition loc_3 : location_info := LocationInfo file_0 8 2 8 13.
+  Definition loc_4 : location_info := LocationInfo file_0 9 2 9 12.
+  Definition loc_5 : location_info := LocationInfo file_0 10 2 10 14.
+  Definition loc_6 : location_info := LocationInfo file_0 11 2 11 13.
+  Definition loc_7 : location_info := LocationInfo file_0 13 2 13 21.
+  Definition loc_8 : location_info := LocationInfo file_0 14 2 14 21.
+  Definition loc_9 : location_info := LocationInfo file_0 15 2 15 21.
+  Definition loc_10 : location_info := LocationInfo file_0 16 2 16 21.
+  Definition loc_11 : location_info := LocationInfo file_0 17 2 17 21.
+  Definition loc_12 : location_info := LocationInfo file_0 19 2 19 17.
+  Definition loc_13 : location_info := LocationInfo file_0 20 2 20 16.
+  Definition loc_14 : location_info := LocationInfo file_0 21 2 21 16.
+  Definition loc_15 : location_info := LocationInfo file_0 22 2 22 16.
+  Definition loc_16 : location_info := LocationInfo file_0 23 2 23 16.
+  Definition loc_17 : location_info := LocationInfo file_0 25 2 25 9.
+  Definition loc_19 : location_info := LocationInfo file_0 23 9 23 16.
+  Definition loc_22 : location_info := LocationInfo file_0 23 5 23 7.
+  Definition loc_24 : location_info := LocationInfo file_0 23 6 23 7.
+  Definition loc_25 : location_info := LocationInfo file_0 23 6 23 7.
+  Definition loc_26 : location_info := LocationInfo file_0 22 9 22 16.
+  Definition loc_29 : location_info := LocationInfo file_0 22 5 22 7.
+  Definition loc_31 : location_info := LocationInfo file_0 22 6 22 7.
+  Definition loc_32 : location_info := LocationInfo file_0 22 6 22 7.
+  Definition loc_33 : location_info := LocationInfo file_0 21 9 21 16.
+  Definition loc_36 : location_info := LocationInfo file_0 21 5 21 7.
+  Definition loc_38 : location_info := LocationInfo file_0 21 6 21 7.
+  Definition loc_39 : location_info := LocationInfo file_0 21 6 21 7.
+  Definition loc_40 : location_info := LocationInfo file_0 20 9 20 16.
+  Definition loc_43 : location_info := LocationInfo file_0 20 5 20 7.
+  Definition loc_45 : location_info := LocationInfo file_0 20 6 20 7.
+  Definition loc_46 : location_info := LocationInfo file_0 20 6 20 7.
+  Definition loc_47 : location_info := LocationInfo file_0 19 10 19 17.
+  Definition loc_50 : location_info := LocationInfo file_0 19 5 19 8.
+  Definition loc_52 : location_info := LocationInfo file_0 19 6 19 8.
+  Definition loc_53 : location_info := LocationInfo file_0 19 6 19 8.
+  Definition loc_54 : location_info := LocationInfo file_0 17 14 17 21.
+  Definition loc_57 : location_info := LocationInfo file_0 17 5 17 12.
+  Definition loc_58 : location_info := LocationInfo file_0 17 5 17 7.
+  Definition loc_59 : location_info := LocationInfo file_0 17 5 17 7.
+  Definition loc_60 : location_info := LocationInfo file_0 17 11 17 12.
+  Definition loc_61 : location_info := LocationInfo file_0 17 11 17 12.
+  Definition loc_62 : location_info := LocationInfo file_0 16 14 16 21.
+  Definition loc_65 : location_info := LocationInfo file_0 16 5 16 12.
+  Definition loc_66 : location_info := LocationInfo file_0 16 5 16 7.
+  Definition loc_67 : location_info := LocationInfo file_0 16 5 16 7.
+  Definition loc_68 : location_info := LocationInfo file_0 16 11 16 12.
+  Definition loc_69 : location_info := LocationInfo file_0 16 11 16 12.
+  Definition loc_70 : location_info := LocationInfo file_0 15 14 15 21.
+  Definition loc_73 : location_info := LocationInfo file_0 15 5 15 12.
+  Definition loc_74 : location_info := LocationInfo file_0 15 5 15 7.
+  Definition loc_75 : location_info := LocationInfo file_0 15 5 15 7.
+  Definition loc_76 : location_info := LocationInfo file_0 15 11 15 12.
+  Definition loc_77 : location_info := LocationInfo file_0 15 11 15 12.
+  Definition loc_78 : location_info := LocationInfo file_0 14 14 14 21.
+  Definition loc_81 : location_info := LocationInfo file_0 14 5 14 12.
+  Definition loc_82 : location_info := LocationInfo file_0 14 5 14 7.
+  Definition loc_83 : location_info := LocationInfo file_0 14 5 14 7.
+  Definition loc_84 : location_info := LocationInfo file_0 14 11 14 12.
+  Definition loc_85 : location_info := LocationInfo file_0 14 11 14 12.
+  Definition loc_86 : location_info := LocationInfo file_0 13 14 13 21.
+  Definition loc_89 : location_info := LocationInfo file_0 13 5 13 12.
+  Definition loc_90 : location_info := LocationInfo file_0 13 5 13 7.
+  Definition loc_91 : location_info := LocationInfo file_0 13 5 13 7.
+  Definition loc_92 : location_info := LocationInfo file_0 13 11 13 12.
+  Definition loc_93 : location_info := LocationInfo file_0 13 11 13 12.
+  Definition loc_94 : location_info := LocationInfo file_0 11 11 11 12.
+  Definition loc_97 : location_info := LocationInfo file_0 10 12 10 13.
+  Definition loc_100 : location_info := LocationInfo file_0 9 10 9 11.
+  Definition loc_103 : location_info := LocationInfo file_0 8 11 8 12.
+  Definition loc_106 : location_info := LocationInfo file_0 7 17 7 18.
+  Definition loc_111 : location_info := LocationInfo file_0 30 2 30 16.
+  Definition loc_112 : location_info := LocationInfo file_0 31 2 31 27.
+  Definition loc_113 : location_info := LocationInfo file_0 32 2 32 64.
+  Definition loc_114 : location_info := LocationInfo file_0 32 9 32 62.
+  Definition loc_115 : location_info := LocationInfo file_0 32 9 32 57.
+  Definition loc_116 : location_info := LocationInfo file_0 32 10 32 34.
+  Definition loc_117 : location_info := LocationInfo file_0 32 10 32 16.
+  Definition loc_118 : location_info := LocationInfo file_0 32 11 32 16.
+  Definition loc_119 : location_info := LocationInfo file_0 32 20 32 34.
+  Definition loc_120 : location_info := LocationInfo file_0 32 37 32 52.
+  Definition loc_121 : location_info := LocationInfo file_0 32 37 32 48.
+  Definition loc_122 : location_info := LocationInfo file_0 32 38 32 39.
+  Definition loc_123 : location_info := LocationInfo file_0 32 42 32 43.
+  Definition loc_124 : location_info := LocationInfo file_0 32 46 32 47.
+  Definition loc_125 : location_info := LocationInfo file_0 32 51 32 52.
+  Definition loc_126 : location_info := LocationInfo file_0 32 55 32 56.
+  Definition loc_127 : location_info := LocationInfo file_0 32 61 32 62.
+  Definition loc_128 : location_info := LocationInfo file_0 31 9 31 25.
+  Definition loc_129 : location_info := LocationInfo file_0 31 9 31 20.
+  Definition loc_130 : location_info := LocationInfo file_0 31 10 31 11.
+  Definition loc_131 : location_info := LocationInfo file_0 31 14 31 15.
+  Definition loc_132 : location_info := LocationInfo file_0 31 18 31 19.
+  Definition loc_133 : location_info := LocationInfo file_0 31 24 31 25.
+  Definition loc_134 : location_info := LocationInfo file_0 30 14 30 15.
 
   (* Definition of function [test1]. *)
   Definition impl_test1 : function := {|
@@ -283,6 +307,38 @@ Section code.
         else
         locinfo: loc_17 ;
           Goto "#12"
+      ]> $∅
+    )%E
+  |}.
+
+  (* Definition of function [test_ternary]. *)
+  Definition impl_test_ternary : function := {|
+    f_args := [
+    ];
+    f_local_vars := [
+      ("local", it_layout i32)
+    ];
+    f_init := "#0";
+    f_code := (
+      <[ "#0" :=
+        "local" <-{ it_layout i32 } LocInfoE loc_134 (i2v 0 i32) ;
+        locinfo: loc_112 ;
+        assert: (LocInfoE loc_128 (UnOp (CastOp $ IntOp bool_it) (IntOp i32) (LocInfoE loc_128 ((LocInfoE loc_129 (IfE
+        (IntOp i32)
+        (LocInfoE loc_130 (i2v 2 i32))
+        (LocInfoE loc_131 (i2v 3 i32))
+        (LocInfoE loc_132 (i2v 2 i32)))) ={IntOp i32, IntOp i32} (LocInfoE loc_133 (i2v 3 i32)))))) ;
+        locinfo: loc_113 ;
+        assert: (LocInfoE loc_114 (UnOp (CastOp $ IntOp bool_it) (IntOp i32) (LocInfoE loc_114 ((LocInfoE loc_115 (IfE
+        (IntOp i32)
+        (LocInfoE loc_116 ((LocInfoE loc_117 (&(LocInfoE loc_118 ("local")))) !={PtrOp, PtrOp} (LocInfoE loc_119 (NULL))))
+        (LocInfoE loc_120 ((LocInfoE loc_121 (IfE
+        (IntOp i32)
+        (LocInfoE loc_122 (i2v 1 i32))
+        (LocInfoE loc_123 (i2v 1 i32))
+        (LocInfoE loc_124 (i2v 0 i32)))) +{IntOp i32, IntOp i32} (LocInfoE loc_125 (i2v 3 i32))))
+        (LocInfoE loc_126 (i2v 2 i32)))) ={IntOp i32, IntOp i32} (LocInfoE loc_127 (i2v 4 i32)))))) ;
+        Return (VOID)
       ]> $∅
     )%E
   |}.
