examples/proofs/tests/generated_proof_test_ternary.v
@@ -1,0 +1,26 @@
+From refinedc.typing Require Import typing.
+From refinedc.examples.tests Require Import generated_code.
+From refinedc.examples.tests Require Import generated_spec.
+Set Default Proof Using "Type".
+
+(* Generated from [examples/tests.c]. *)
+Section proof_test_ternary.
+  Context `{!typeG Σ} `{!globalG Σ}.
+
+  (* Typing proof for [test_ternary]. *)
+  Lemma type_test_ternary :
+    ⊢ typed_function impl_test_ternary type_of_test_ternary.
+  Proof.
+    Open Scope printing_sugar.
+    start_function "test_ternary" ([]) => local_local.
+    split_blocks ((
+      ∅
+    )%I : gmap label (iProp Σ)) ((
+      ∅
+    )%I : gmap label (iProp Σ)).
+    - repeat liRStep; liShow.
+      all: print_typesystem_goal "test_ternary" "#0".
+    Unshelve. all: sidecond_hook; prepare_sideconditions; normalize_and_simpl_goal; try solve_goal; unsolved_sidecond_hook.
+    all: print_sidecondition_goal "test_ternary".
+  Qed.
+End proof_test_ternary.
